Added order lowering for taylor models.

Poly_Ex.thy
@@ -25,7 +25,7 @@ value "Ipoly [Ivl (Float 4 (-6)) (Float 10 6)] (poly.Add (poly.C (Float 3 5)) (p
 
 (* Coercing a "float poly" into a "real poly" is a homomorphism. *)
 lemma poly_map_real_polyadd:
-fixes p1::"float poly"
+fixes p1 p2 :: "float poly"
 shows "poly_map real (p1 +\<^sub>p p2) = poly_map real p1 +\<^sub>p poly_map real p2"
 apply(induction p1 arbitrary: p2)
 apply(simp_all)[7]
@@ -51,9 +51,19 @@ next
       by (simp_all add: real_of_float_eq 2[symmetric])
     qed
 qed
+
+lemma poly_map_real_polyneg:
+fixes p :: "float poly"
+shows "poly_map real (~\<^sub>pp) = ~\<^sub>p(poly_map real p)"
+by (induction p) simp_all
+
+lemma poly_map_real_polysub:
+fixes p1 p2 :: "float poly"
+shows "poly_map real (p1 -\<^sub>p p2) = poly_map real p1 -\<^sub>p poly_map real p2"
+by (simp add: polysub_def poly_map_real_polyadd poly_map_real_polyneg)
     
 lemma poly_map_real_polymul:
-fixes p1::"float poly"
+fixes p1 p2 :: "float poly"
 shows "poly_map real (p1 *\<^sub>p p2) = poly_map real p1 *\<^sub>p poly_map real p2"
 apply(induction p1 arbitrary: p2)
 apply(simp_all)[7]
@@ -82,6 +92,19 @@ next
     qed
 qed
 
+lemma poly_map_real_polypow:
+fixes p :: "float poly"
+shows "poly_map real (p^\<^sub>pn) = (poly_map real p)^\<^sub>pn"
+proof(induction n rule: nat_less_induct)
+  fix n assume assm: "\<forall>m<n. poly_map real (p ^\<^sub>p m) = (poly_map real) p ^\<^sub>p m"
+  thus "poly_map real (p ^\<^sub>p n) = poly_map real p ^\<^sub>p n"
+    apply(cases n)
+    apply(simp_all)
+    by (smt Suc_less_eq div2_less_self even_Suc odd_Suc_div_two poly_map_real_polymul)
+qed
+
+lemmas poly_map_real_polyarith = poly_map_real_polyadd poly_map_real_polyneg poly_map_real_polysub poly_map_real_polymul poly_map_real_polypow
+
 (* Count the number of parameters of a polynomial. *)
 fun num_params :: "'a poly \<Rightarrow> nat"
 where "num_params (poly.C c) = 0"
@@ -93,29 +116,118 @@ where "num_params (poly.C c) = 0"
     | "num_params (poly.Pw a n)   = num_params a"
     | "num_params (poly.CN a n b) = max (max (num_params a) (num_params b)) (Suc n)"
     
-lemma [simp]: "num_params (poly_map real p) = num_params p"
+lemma num_params_poly_map_real[simp]:
+shows "num_params (poly_map real p) = num_params p"
 by (induction p, simp_all)
 
+lemma num_params_polyadd:
+shows "num_params (p1 +\<^sub>p p2) \<le> max (num_params p1) (num_params p2)"
+apply(induction p1 p2 rule: polyadd.induct)
+apply(auto)[3]
+proof-
+  case (4 c n p c' n' p')
+  show ?case
+    apply(cases "n' < n")
+    apply(simp)
+    using 4
+    apply(simp)
+    apply(smt max.cobounded2 max.coboundedI2 max.commute max_def)
+    apply(cases "n' = n")
+    apply(simp add: Let_def)
+    apply(smt "4.IH"(3) "4.IH"(4) le_max_iff_disj max.cobounded1)
+    apply(simp)
+    apply(safe)
+    apply(simp_all)
+    using 4(1) by auto
+qed simp_all
+
+lemma num_params_polyneg:
+shows "num_params (~\<^sub>p p) = num_params p"
+by (induction p rule: polyneg.induct) simp_all
+
+lemma num_params_polymul:
+shows "num_params (p1 *\<^sub>p p2) \<le> max (num_params p1) (num_params p2)"
+apply(induction p1 p2 rule: polymul.induct)
+apply(auto)[3]
+proof-
+  case (4 c n p c' n' p')
+  show ?case
+    apply(cases "n' < n")
+    apply(simp)
+    using 4
+    apply(simp)
+    apply(smt max.cobounded2 max.coboundedI2 max.commute max_def)
+    apply(cases "n' > n")
+    apply(simp add: Let_def)
+    apply(safe)
+    apply(simp_all)
+    using 4(1)
+    apply auto[1]
+    using 4(2)
+    apply(smt le_SucI le_neq_implies_less le_refl le_trans less_Suc_eq_le less_eq_Suc_le less_max_iff_disj less_not_refl linorder_neqE_nat max.absorb1 max.absorb2 max.assoc max.bounded_iff max.cobounded2 max.coboundedI1 max.coboundedI2 max.commute max.left_commute max.strict_order_iff max_less_iff_conj nat_le_linear not_less_eq_eq num_params.simps(8))
+    using 4(3,4) num_params_polyadd[of "CN c n p *\<^sub>p c'" "CN 0\<^sub>p n (CN c n p *\<^sub>p p')"]
+    apply(simp)
+    by (smt max.commute max.left_commute max_def)
+qed simp_all
+
+lemma num_params_polypow:
+shows "num_params (p ^\<^sub>p n) \<le> num_params p"
+using assms
+apply(induction n rule: polypow.induct)
+apply(simp)
+proof-
+  fix v assume "(\<And>x. num_params (p ^\<^sub>p Suc v div 2) \<le> num_params p)"
+  thus "num_params (p ^\<^sub>p Suc v) \<le> num_params p"
+    unfolding polypow.simps
+    apply(simp add: Let_def del: polypow.simps)
+    apply(safe)
+    apply(smt Suc_eq_plus1 add_self_div_2 dvd.order.trans evenE even_Suc even_Suc_div_two even_numeral max_def mult.commute mult_2 num_params_polymul oddE odd_Suc_div_two order.trans order_refl)
+    by (smt even_Suc_div_two le_max_iff_disj max_def num_params_polymul)
+qed
+
+find_theorems "linorder_class.Max (_ \<union> _)"
+find_theorems "0::nat" name: "induct"
+
+lemma num_params_polynate:
+shows "num_params (polynate p) \<le> num_params p"
+proof(induction p rule: polynate.induct)
+  case (2 l r)
+  thus ?case
+    using num_params_polyadd[of "polynate l" "polynate r"]
+    by simp
+next
+  case (3 l r)
+  thus ?case
+    apply(simp add: polysub_def)
+    using num_params_polyadd[of "polynate l" "~\<^sub>p (polynate r)"] 
+    by (simp add: num_params_polyneg)
+next
+  case (4 l r)
+  thus ?case
+    using num_params_polymul[of "polynate l" "polynate r"]
+    by simp
+next
+  case (5 p)
+  thus ?case
+    by (simp add: num_params_polyneg)
+next
+  case (6 p n)
+  thus ?case
+    using num_params_polypow[of n "polynate p"]
+    by simp
+qed simp_all
+
+lemma polynate_poly_map_real[simp]:
+fixes p :: "float poly"
+shows "poly_map real (polynate p) = polynate (poly_map real p)"
+by (induction p) (simp_all add: poly_map_real_polyarith)
+                                      
 (* Evaluating a float poly is equivalent to evaluating the corresponding
    real poly with the float parameters converted to reals. *)
 lemma Ipoly_real_float_eqiv:
 fixes p::"float poly" and xs::"float list"
 assumes "num_params p \<le> length xs"
 shows "Ipoly xs (p::real poly) = Ipoly xs p"
-using assms by (induction p, simp_all)
-
-lemma Ipoly_real_float_interval_eqiv:
-fixes p::"float interval poly" and xs::"float interval list"
-assumes "num_params p \<le> length xs"
-shows "Ipoly (map (interval_map real) xs) (poly_map (interval_map real) p) = interval_map real (Ipoly xs p)"
-using assms by (induction p, simp_all)
-
-
-(* TODO: This lemma is a mess and similar to Ipoly_real_float_interval_eqiv. *)
-lemma Ipoly_real_float_interval_eqiv':
-fixes p::"float poly" and xs::"float interval list"
-assumes "num_params p \<le> length xs"
-shows "Ipoly (map (interval_map real) xs) (poly_map interval_of (poly_map real p)) = interval_map real (Ipoly xs (poly_map interval_of p))"
 using assms by (induction p, simp_all)
 
 (* Evaluating an "'a poly" with "'a interval" arguments is monotone. *)
@@ -140,5 +252,169 @@ using assms(1)
 apply(induction p)
 using assms(2)
 by (simp_all add: set_of_add_inc set_of_sub_inc set_of_mul_inc set_of_neg_inc set_of_pow_inc)
+
+section \<open>Splitting polynomials to reduce floating point precision\<close>
+
+(* TODO: Move this! Definitions regarding floating point numbers should not be in a theory about polynomials. *)
+fun float_prec :: "float \<Rightarrow> int"
+where "float_prec f = (let p=exponent f in if p \<ge> 0 then 0 else -p)"
+
+fun float_round :: "nat \<Rightarrow> float \<Rightarrow> float"
+where "float_round prec f = (
+         let d = float_down prec f; u = float_up prec f
+         in if f - d < u - f then d else u)"
+
+lemma float_round_correct:
+shows "float_prec (float_round prec f) \<le> prec"
+apply(cases f)
+apply(simp add: Let_def, safe)
+thm float_down_correct
+oops
+
+(* Splits any polynomial p into two polynomials l, r, such that for all x::real. p(x) = l(x) + r(x)
+   and all floating point coefficients in p are rounded to precision prec.
+   Not all cases need to be give good results. Polynomials normalized with polynate
+   only contain poly.C and poly.CN constructors. *)
+fun split_by_prec :: "nat \<Rightarrow> float poly \<Rightarrow> float poly * float poly"
+where "split_by_prec prec (poly.C f) = (let r = float_round prec f in (poly.C r, poly.C (f - r)))"
+    | "split_by_prec prec (poly.Bound n) = (poly.Bound n, poly.C 0)"
+    | "split_by_prec prec (poly.Add l r) = (let (ll, lr) = split_by_prec prec l;
+                                                (rl, rr) = split_by_prec prec r
+                                            in (poly.Add ll rl, poly.Add lr rr))"
+    | "split_by_prec prec (poly.Sub l r) = (let (ll, lr) = split_by_prec prec l;
+                                             (rl, rr) = split_by_prec prec r
+                                         in (poly.Sub ll rl, poly.Sub lr rr))"
+    | "split_by_prec prec (poly.Mul l r) = (let (ll, lr) = split_by_prec prec l;
+                                                (rl, rr) = split_by_prec prec r
+                                            in (poly.Mul ll rl, poly.Add (poly.Add (poly.Mul lr rl) (poly.Mul ll rr)) (poly.Mul lr rr)))"
+    | "split_by_prec prec (poly.Neg p) = (let (l, r) = split_by_prec prec p in (poly.Neg l, poly.Neg r))"
+    | "split_by_prec prec (poly.Pw p 0) = (poly.C 1, poly.C 0)"
+    | "split_by_prec prec (poly.Pw p (Suc n)) = (let (l, r) = split_by_prec prec p in (poly.Pw l n, poly.Sub (poly.Pw p (Suc n)) (poly.Pw l n)))"
+    | "split_by_prec prec (poly.CN c n p) = (let (cl, cr) = split_by_prec prec c;
+                                                 (pl, pr) = split_by_prec prec p
+                                             in (poly.CN cl n pl, poly.CN cr n pr))"
+
+(* TODO: Prove precision constraint on l. *)
+lemma split_by_prec_correct:
+fixes args :: "real list"
+assumes "(l, r) = split_by_prec prec p"
+shows "Ipoly args p = Ipoly args l + Ipoly args r"
+using assms
+proof(induction p arbitrary: l r)
+  case (Add p1 p2 l r)
+  thus ?case by (simp add: Add(1,2)[OF pair_collapse] split_beta)
+next
+  case (Sub p1 p2 l r)
+  thus ?case by (simp add: Sub(1,2)[OF pair_collapse] split_beta)
+next
+  case (Mul p1 p2 l r)
+  thus ?case by (simp add: Mul(1,2)[OF pair_collapse] split_beta algebra_simps)
+next
+  case (Neg p l r) 
+  thus ?case by (simp add: Neg(1)[OF pair_collapse] split_beta)
+next
+  case (Pw p n l r)
+  thus ?case by (cases n) (simp_all add: Pw(1)[OF pair_collapse] split_beta)
+next
+  case (CN c n p2)
+  thus ?case by (simp add: CN(1,2)[OF pair_collapse] split_beta algebra_simps)
+qed (simp_all add: Let_def)
+
+section \<open>Splitting polynomials by degree\<close>
+
+fun maxdegree :: "('a::zero) poly \<Rightarrow> nat"
+where "maxdegree (poly.C c) = 0"
+    | "maxdegree (poly.Bound n) = 1"
+    | "maxdegree (poly.Add l r) = max (maxdegree l) (maxdegree r)"
+    | "maxdegree (poly.Sub l r) = max (maxdegree l) (maxdegree r)"
+    | "maxdegree (poly.Mul l r) = maxdegree l + maxdegree r"
+    | "maxdegree (poly.Neg p) = maxdegree p"
+    | "maxdegree (poly.Pw p n) = n * maxdegree p"
+    | "maxdegree (poly.CN c n p) = max (maxdegree c) (1 + maxdegree p)"
+
+fun split_by_degree :: "nat \<Rightarrow> 'a::zero poly \<Rightarrow> 'a poly * 'a poly"
+where "split_by_degree n (poly.C c) = (poly.C c, poly.C 0)"
+    | "split_by_degree 0 p = (poly.C 0, p)"
+    | "split_by_degree (Suc n) (poly.CN c v p) = (
+         let (cl, cr) = split_by_degree (Suc n) c;
+             (pl, pr) = split_by_degree n p
+         in (poly.CN cl v pl, poly.CN cr v pr))"
+    (* This function is only intended for use on polynomials in normal form.
+       Hence most cases never get executed. *)
+    | "split_by_degree n p = (poly.C 0, p)"
+
+lemma split_by_degree_correct:
+fixes x :: "real list" and p :: "float poly"
+assumes "(l, r) = split_by_degree n p"
+shows "maxdegree l \<le> n" (is ?P1)
+and   "Ipoly x p = Ipoly x l + Ipoly x r" (is ?P2)
+and   "num_params l \<le> num_params p" (is ?P3)
+and   "num_params r \<le> num_params p" (is ?P4)
+proof-
+  have proposition: "?P1 \<and> ?P2 \<and> ?P3 \<and> ?P4"
+  using assms
+  proof(induction p arbitrary: l r n)
+    case (C c l r n)
+    thus ?case by simp
+  next
+    case (Bound v l r n)
+    thus ?case by (cases n) simp_all
+  next
+    case (Add p1 p2 l r n)
+    thus ?case by (cases n) simp_all
+  next
+    case (Sub p1 p2 l r n)
+    thus ?case by (cases n) simp_all
+  next
+    case (Mul p1 p2 l r n)
+    thus ?case by (cases n) simp_all
+  next
+    case (Neg p l r n)
+    thus ?case by (cases n) simp_all
+  next
+    case (Pw p k l r n)
+    thus ?case by (cases n) simp_all
+  next
+    case (CN c v p l r n)
+    show ?case
+    proof(cases n)
+      case 0
+      thus ?thesis using CN by simp
+    next
+      case (Suc m)
+      obtain cl cr where cl_cr_def: "(cl, cr) = split_by_degree (Suc m) c"
+        by (cases "split_by_degree (Suc m) c", simp)
+      obtain pl pr where pl_pr_def: "(pl, pr) = split_by_degree m p"
+        by (cases "split_by_degree m p", simp)
+      have [simp]: "Ipoly x p = Ipoly x pl + Ipoly x pr"
+        using CN(2)[OF pl_pr_def]
+        by (cases n) simp_all
+      from CN(3)
+      have l_decomp: "l = CN cl v pl" and r_decomp: "r = CN cr v pr"
+        by (simp_all add: Suc cl_cr_def[symmetric] pl_pr_def[symmetric])
+      show ?thesis
+        apply(simp add: l_decomp, safe)
+        using CN(1)[OF cl_cr_def]
+        apply(simp add: Suc)
+        using CN(2)[OF pl_pr_def]
+        apply(simp add: Suc)
+        using pl_pr_def
+        apply(cases p)
+        apply(simp_all)
+        apply(simp_all add: l_decomp r_decomp CN(1)[OF cl_cr_def] algebra_simps)
+        apply(safe)
+        prefer 3
+        using CN(1)[OF cl_cr_def] 
+        apply(simp_all add: max.coboundedI1)[2]
+        using CN(2)[OF pl_pr_def]
+        by auto
+    qed
+  qed
+  
+  show ?P1 using proposition by simp
+  show ?P2 using proposition by simp
+  show ?P3 using proposition by simp
+  show ?P4 using proposition by simp
+qed
 
 end
